src/meta/expr.lean
@@ -666,3 +666,7 @@ meta def univ_levels (d : declaration) : list level :=
 d.univ_params.map level.param
 
 end declaration
+
+meta instance pexpr.decidable_eq : decidable_eq pexpr :=
+unchecked_cast
+expr.has_decidable_eq
